src/syntax.lean
@@ -9,53 +9,52 @@ class names (α : Type) :=
 (Nf {x : α} (H: x ∈ Nc): finset α)
 (Nm {x : α} (H: x ∈ Nc): finset α)
 (Np {x : α} {H: x ∈ Nc} {y : α} (G : y ∈ Nm H): finset α)
-section open names variables {α : Type} [names α]
-  structure class_name (α : Type) [names α] :=
-    (name : α) (H : name ∈ Nc α)
-  section variables (self : class_name α)
-    structure field_name :=
-      (name : α) (G: name ∈ Nf self.H)
-    structure method_name :=
-      (name : α) (G: name ∈ Nm self.H)
-  end
-  variable {self : class_name α}
-  structure param_name (m : method_name self) :=
-    (name : α) (F: name ∈ Np m.G)
-end
 
-/- A type in our object language is either: a reference type (by class name), or a data type from the host language. A variable context is a list of types; a local variable is encoded by an index in this context. Local variables do not have a name. -/
-section variables (α : Type) [names α]
-  inductive type
+section variables {α : Type} [names α]
+  section open names
+    structure class_name (α : Type) [names α] :=
+      (name : α) (H : name ∈ Nc α)
+    section variables (self : class_name α)
+      structure field_name :=
+        (name : α) (G: name ∈ Nf self.H)
+      structure method_name :=
+        (name : α) (G: name ∈ Nm self.H)
+    end
+    variable {self : class_name α}
+    structure param_name (m : method_name self) :=
+      (name : α) (F: name ∈ Np m.G)
+  end
+  /- A type in our object language is either: a reference type (by class name), or a data type from the host language. A variable context is a list of types; a local variable is encoded by an index in this context. Local variables do not have a name. -/
+  inductive type (α : Type) [names α]
   | ref: class_name α → type
   | data: Type → type
   instance : has_coe Type (type α) := ⟨type.data α⟩
-  @[reducible] def context := list (type α)
-end
-open type
+  /- A local variable context is a list of types. -/
+  @[reducible] def context (α : Type) [names α] := list (type α)
 
-/- A program signature consists of: a map from class names to class declarations, and a class name of the root object. A class declaration (of some class self) consists of a map from field names to field declarations, a map from method names to method declarations, and a method name that indicates a constructor. A field declaration consists of a type. A method declaration consists of a map from parameter names to parameter declarations. A parameter declaration consists of a type. -/
-section variables {α : Type} [names α]
-    {self : class_name α}
-    {m : method_name self}
-  structure pdecl (p : param_name m) :=
-    (type : type α)
-  structure mdecl (m : method_name self) :=
-    (pdecl (p : param_name m) : pdecl p)
-  structure fdecl (f : field_name self) :=
-    (type : type α)
-  structure cdecl (self : class_name α) :=
-    (fdecl (f : field_name self) : fdecl f)
-    (mdecl (m : method_name self) : mdecl m)
-    (ctor : method_name self)
--- Design choice: constructors and methods are treated uniformly.
+  /- A program signature consists of: a map from class names to class declarations, and a class name of the root object. A class declaration (of some class self) consists of a map from field names to field declarations, a map from method names to method declarations, and a method name that indicates a constructor. A field declaration consists of a type. A method declaration consists of a map from parameter names to parameter declarations. A parameter declaration consists of a type. -/
+  section variables {self : class_name α} {m : method_name self}
+    structure pdecl (p : param_name m) :=
+      (type : type α)
+    structure mdecl (m : method_name self) :=
+      (pdecl (p : param_name m) : pdecl p)
+    structure fdecl (f : field_name self) :=
+      (type : type α)
+    structure cdecl (self : class_name α) :=
+      (fdecl (f : field_name self) : fdecl f)
+      (mdecl (m : method_name self) : mdecl m)
+      (ctor : method_name self)
+  -- Design choice: constructors and methods are treated uniformly.
+  end
 end
 
 class signature (α : Type) extends names α : Type 1 :=
 (cdef (x : class_name α): cdecl x) (main: class_name α)
 
-section variables {α : Type} [signature α]
-    {self : class_name α}
-    {m : method_name self}
+variables {α : Type} [signature α]
+open type
+
+section variables {self : class_name α} {m : method_name self}
   def param_type (p : param_name m) : type α :=
     (((signature.cdef self).mdecl m).pdecl p).type
   def field_type (f : field_name self) : type α :=
@@ -73,7 +72,7 @@ structure tenv (α : Type) [signature α] : Type 1 :=
 /- A note on terminology. Parameter: as declared in signature. Argument: a pure expression as supplied in a method call. -/
 
 /- Within a typing environment, we refer to numerous things. This refers to an object identity of the enclosed class. A local variable refers to the index within the declared local variables. A parameter refers to a parameter name of the current method. A field refers to a field within the enclosed class. -/
-section variables {α : Type} [signature α] (e : tenv α)
+section variable (e : tenv α)
   section variable (ty : type α)
     structure tvar := (H : ty = ref e.self)
     structure lvar := (idx : list_at ty e.locals)
@@ -94,7 +93,7 @@ section variables {α : Type} [signature α] (e : tenv α)
   end
   /- A pure expression within a typing environment is either: a constant data value, a function application on data values, value lookup in environment, referential equality check. -/
   inductive pexp : type α → Type 1
-  | value {γ : Type}: γ → pexp γ
+  | const {γ : Type}: γ → pexp γ
   | apply {γ δ : Type}: pexp (γ → δ) → pexp γ → pexp δ
   | lookup {ty : type α}: rvar e ty → pexp ty
   | requal {c : class_name α}:
@@ -118,11 +117,8 @@ section variables {α : Type} [signature α] (e : tenv α)
 end
 
 /- A program with a given program signature associates to each method of each class a program block. A program block associated to a method consists of: local variable declarations, and a statement within a typing environment. -/
-section variables {α : Type} [signature α]
-  structure pblock {self : class_name α}
-      (m : method_name self) :=
-    (locals : context α)
-    (S : stmt (tenv.mk self m locals))
-  structure program :=
-    (body {self : class_name α} (m : method_name self): pblock m)
-end
+structure pblock {self : class_name α} (m : method_name self) :=
+  (locals : context α)
+  (S : stmt (tenv.mk self m locals))
+structure program :=
+  (body {self : class_name α} (m : method_name self): pblock m)
